concur/VCompNew.v
@@ -1,0 +1,252 @@
+Require Export LogicalRelations.
+Require Export List.
+Require Export Globalenvs.
+Require Export Events.
+Require Export LanguageInterface.
+Require Export Smallstep.
+
+Require Import Axioms.
+Require Import Coqlib.
+Require Import Integers.
+Require Import Values.
+Require Import Memory.
+
+Require Import CallconvNew.
+
+Require Import RelClasses.
+
+
+(* Set Asymmetric Patterns. *)
+(* Set Implicit Arguments. *)
+ Generalizable All Variables. 
+
+Import GS.
+
+
+Section COMP_FSIM.
+
+  Context `(cc1: callconv lis lin) `(cc2: callconv lin lif)
+          (Ls: semantics lis lis) (Ln: semantics lin lin) (Lf: semantics lif lif).
+  Context (H1: fsim_components cc1 Ls Ln)
+          (H2: fsim_components cc2 Ln Lf).
+
+  Inductive compose_fsim_match_states se1 se3:
+    ccworld (cc_compose cc1 cc2) ->
+    gworld (cc_compose cc1 cc2) ->
+    (fsim_index H2 * fsim_index H1) ->
+    state Ls -> state Lf -> Prop :=
+  | compose_match_states_intro se2 s1 s2 s3 i1 i2 wb1 wb2 wp1 wp2
+    (HS1: fsim_match_states H1 se1 se2 wb1 wp1 i1 s1 s2)
+    (HS2: fsim_match_states H2 se2 se3 wb2 wp2 i2 s2 s3):
+    compose_fsim_match_states se1 se3 (se2, (wb1, wb2)) (wp1,wp2) (i2, i1) s1 s3.
+
+  (** Is this necessary or useful? *)
+  (*Inductive compose_fsim_inv:
+    gworld (cc_compose cc1 cc2) -> gworld (cc_compose cc1 cc2) -> Prop :=
+  | compose_fsim_inv_intro wa1 wa2 wb1 wb2
+      (INV1: fsim_invariant H1 wa1 wb1)
+      (INV2: fsim_invariant H2 wa2 wb2):
+    compose_fsim_inv (wa1, wa2) (wb1, wb2).*)
+
+  Lemma st_fsim_vcomp':
+    fsim_components (cc_compose cc1 cc2) Ls Lf.
+  Proof.
+    set (ff_order := lex_ord (Relation_Operators.clos_trans
+                                _ (fsim_order H2)) (fsim_order H1)).
+    apply GS.Forward_simulation with ff_order compose_fsim_match_states.
+    - rewrite (fsim_skel H1); apply (fsim_skel H2).
+    - intros se1 se3 [se2 [wb1 wb2]] [Hse01 Hse02] Hse1.
+      pose proof (@fsim_lts _ _ _ _ _ H1 se1 se2 wb1 Hse01 Hse1) as X1.
+      assert (Hse2: Genv.valid_for (skel Ln) se2).
+      { rewrite <- (fsim_skel H1). eapply match_senv_valid_for; eauto. }
+      pose proof (@fsim_lts _ _ _ _ _ H2 se2 se3 wb2 Hse02 Hse2) as X2.
+      clear Hse1 Hse2. constructor.
+      + intros q1 q3 (q2 & Hq1 & Hq2).
+        etransitivity; eauto using fsim_match_valid_query.
+      + intros q1 q3 s1 (q2 & Hq12 & Hq23) Hi Hse.
+        destruct Hse as (Hse1 & Hse2). cbn in *.
+        edestruct (@fsim_match_initial_states lis) as (i & s2 & A & B); eauto.
+        edestruct (@fsim_match_initial_states lin) as (i' & s3 & C & D); eauto.
+        eexists (i', i), s3. split; eauto.
+        econstructor; eauto.
+      + intros (wb1' & wb2') (i2, i1) s1 s3 r1 Hs H.
+        inv Hs.
+        edestruct (@fsim_match_final_states lis) as (r2 & Hr2 & A); eauto.
+        edestruct (@fsim_match_final_states lin) as (r3 & Hr3 & B); eauto.
+        destruct A as (R1 & I1).
+        destruct B as (R2 & I2).
+        exists r3. repeat split; eauto.
+        econstructor; eauto.
+      + intros (wb1' & wb2') (i2, i1) s1 s3 q1 Hs H.
+        inv Hs.
+        edestruct (@fsim_match_external lis)
+          as (wa2 & q2 & Hq2 & ACC2 & Hq12 & HSE12 & Hk12); eauto.
+        edestruct (@fsim_match_external lin)
+          as (wa3 & q3 & Hq3 & ACC3 & Hq23 & HSE23 & Hk23); eauto.
+        exists (se2, (wa2,wa3)), q3. repeat split; eauto. 
+        * econstructor; eauto.
+        * intros r1 r3 s1' (wpi & wpj) Hw (r2 & Hr12 & Hr23) HH. inv Hw. cbn in *.
+          edestruct Hk12 as (i2' & s2' & Hs2' & wpi' & Hpiw & Hm); eauto.
+          edestruct Hk23 as (i1' & s3' & Hs3' & wpk' & Hpjw & Hn); eauto.
+          eexists (_, _), _. repeat split; eauto.
+          eexists (_, _).
+          repeat split; eauto.
+          econstructor; eauto.
+      + intros s1 t s1' Hstep (wpi & wpj) (i2, i1) s3 Hs.
+        inv Hs.
+        edestruct (@fsim_simulation' lis) as (i1' & wpi' & Hpi & Hx); eauto.
+        destruct Hx as [[s2' [A B]] | [A [B C]]].
+        * (* L2 makes one or several steps. *)
+          edestruct (@simulation_plus lin) as (wpj' & i2' & Hw & Hx); eauto.
+          destruct Hx as [[s3' [P Q]] | [P [Q R]]].
+          -- (* L3 makes one or several steps *)
+            exists (i2', i1'); exists s3'; split.
+            left; eauto.
+            eexists (_, _). repeat split; eauto.
+            econstructor; eauto.
+          -- (* L3 makes no step *)
+            exists (i2', i1'); exists s3; split.
+            right; split. subst t; apply star_refl. red. left. auto.
+            eexists (_, _). repeat split; eauto.
+            econstructor; eauto.
+        * (* L2 makes no step *)
+          exists (i2, i1'); exists s3; split.
+          right; split. subst t; apply star_refl. red. right. auto.
+          eexists (_, _). repeat split; eauto.
+          cbn; reflexivity.
+          econstructor; eauto.
+    - unfold ff_order.
+      apply wf_lex_ord. apply Transitive_Closure.wf_clos_trans.
+      eapply (fsim_order_wf H2). eapply (fsim_order_wf H1).
+  Qed.
+
+End COMP_FSIM.
+
+Lemma st_fsim_vcomp
+  `(cc1: callconv lis lin) `(cc2: callconv lin lif)
+  (Ls: semantics lis lis) (Ln: semantics lin lin) (Lf: semantics lif lif):
+  forward_simulation cc1 Ls Ln ->
+  forward_simulation cc2 Ln Lf ->
+  forward_simulation (cc_compose cc1 cc2) Ls Lf.
+Proof.
+  intros [X] [Y]. constructor. eapply st_fsim_vcomp'; eauto.
+Qed.
+
+
+(** ** Identity *)
+Program Instance world_unit : World unit :=
+  {|
+    w_state := unit;
+    w_lens := lens_id;
+    w_acci := fun _ _ => True;
+    w_acce := fun _ _ => True;
+  |}.
+
+Program Definition cc_id {li}: callconv li li :=
+  {|
+    ccworld := unit;
+    ccworld_world := world_unit;
+    match_senv w := eq;
+    match_query w := eq;
+    match_reply w := eq;
+  |}.
+
+Solve All Obligations with
+  cbn; intros; subst; auto.
+
+Notation "1" := cc_id : gs_cc_scope.
+
+
+(** Algebraic structures on calling conventions. *)
+
+(** * Refinement and equivalence *)
+
+(** ** Definition *)
+
+(** The following relation asserts that the calling convention [cc] is
+  refined by the calling convention [cc'], meaning that any
+  [cc']-simulation is also a [cc]-simulation. *)
+
+Definition ccref {li1 li2} (cc cc': callconv li1 li2) :=
+  forall w se1 se2 q1 q2,
+    match_senv cc w se1 se2 ->
+    match_query cc w q1 q2 ->
+    exists w',
+      match_senv cc' w' se1 se2 /\
+      match_query cc' w' q1 q2 /\
+      forall r1 r2,
+        match_reply cc' w' r1 r2 ->
+        match_reply cc w r1 r2.
+
+Definition cceqv {li1 li2} (cc cc': callconv li1 li2) :=
+  ccref cc cc' /\ ccref cc' cc.
+
+Global Instance ccref_preo li1 li2:
+  PreOrder (@ccref li1 li2).
+Proof.
+  split.
+  - intros cc w q1 q2 Hq.
+    eauto.
+  - intros cc cc' cc'' H' H'' w se1 se2 q1 q2 Hse Hq.
+    edestruct H' as (w' & Hse' & Hq' & Hr'); eauto.
+    edestruct H'' as (w'' & Hse'' & Hq'' & Hr''); eauto 10.
+Qed.
+
+Global Instance cceqv_equiv li1 li2:
+  Equivalence (@cceqv li1 li2).
+Proof.
+  split.
+  - intros cc.
+    split; reflexivity.
+  - intros cc1 cc2. unfold cceqv.
+    tauto.
+  - intros cc1 cc2 cc3 [H12 H21] [H23 H32].
+    split; etransitivity; eauto.
+Qed.
+
+Global Instance ccref_po li1 li2:
+  PartialOrder (@cceqv li1 li2) (@ccref li1 li2).
+Proof.
+  firstorder.
+Qed.
+
+(** ** Relation to forward simulations *)
+
+Global Instance open_fsim_ccref:
+  Monotonic
+    (@forward_simulation)
+    (forallr - @ liA1, forallr - @ liA2, ccref ++>
+     forallr - @ liB1, forallr - @ liB2, ccref -->
+     subrel).
+Proof.
+  
+  intros liA1 liA2 ccA ccA' HA liB1 liB2 ccB ccB' HB sem1 sem2 [FS].
+  destruct FS as [index order match_states SKEL PROP WF].
+  constructor.
+  set (ms se1 se2 w' idx s1 s2 :=
+         exists w : ccworld ccB,
+           match_states se1 se2 w idx s1 s2 /\
+           match_senv ccB w se1 se2 /\
+           forall r1 r2, match_reply ccB w r1 r2 -> match_reply ccB' w' r1 r2).
+  eapply Forward_simulation with order ms; auto.
+  intros se1 se2 wB' Hse' Hse1.
+  split.
+  - intros q1 q2 Hq'.
+    destruct (HB wB' se1 se2 q1 q2) as (wB & Hse & Hq & Hr); auto.
+    eapply fsim_match_valid_query; eauto.
+  - intros q1 q2 s1 Hq' Hs1.
+    destruct (HB wB' se1 se2 q1 q2) as (wB & Hse & Hq & Hr); auto.
+    edestruct @fsim_match_initial_states as (i & s2 & Hs2 & Hs); eauto.
+    exists i, s2. split; auto. exists wB; auto.
+  - intros i s1 s2 r1 (wB & Hs & Hse & Hr') Hr1.
+    edestruct @fsim_match_final_states as (r2 & Hr2 & Hr); eauto.
+  - intros i s1 s2 qA1 (wB & Hs & Hse & Hr') HqA1.
+    edestruct @fsim_match_external as (wA & qA2 & HqA2 & HqA & HseA & ?); eauto.
+    edestruct HA as (wA' & HseA' & HqA' & Hr); eauto.
+    exists wA', qA2. intuition auto.
+    edestruct H as (i' & s2' & Hs2' & Hs'); eauto.
+    exists i', s2'. split; auto. exists wB; eauto.
+  - intros s1 t s1' Hs1' i s2 (wB & Hs & Hse & Hr').
+    edestruct @fsim_simulation as (i' & s2' & Hs2' & Hs'); eauto.
+    exists i', s2'. split; auto. exists wB; eauto.
+Qed.
